Fixed error in sbDom of innerSum4SPF Continued proof

SPF_NewFeedback_MW.thy
@@ -3,21 +3,217 @@ imports "CaseStudies/StreamCase_Study" SPF_Comp SPF_Templates SPF_FeedComp SPF_F
 
 begin
 
-section \<open> general lemmas about sercomp and parcomp \<close>  
+section \<open>Feedback Definitions\<close>
+
+
+definition mapIdFunct :: "(channel \<rightharpoonup> channel) \<Rightarrow> channel \<Rightarrow> channel" where
+"mapIdFunct m \<equiv> (\<lambda> c. case m c of None \<Rightarrow> c | Some y \<Rightarrow> y )" 
+ 
+definition map_inverse :: "(channel \<rightharpoonup> channel) \<Rightarrow> (channel \<rightharpoonup> channel)" where
+"map_inverse m \<equiv> (\<lambda>x. if (x \<in> (ran m)) then Some ((\<lambda> y. (THE z. m z = Some y)) x) else None)"
+    
+definition sbRenameChMap :: "'m SB \<Rightarrow> (channel \<rightharpoonup> channel) \<Rightarrow> 'm SB" where
+"sbRenameChMap sb m \<equiv> Abs_SB (\<lambda>c. if (c \<in> (sbDom\<cdot>sb \<inter> dom(m) - ran(m))) then None else Rep_SB(sb)((mapIdFunct (map_inverse m))(c)))"  
+  
+definition spfRename :: "'a SPF \<Rightarrow> (channel \<rightharpoonup> channel) \<Rightarrow> 'a SPF" where
+"spfRename f m \<equiv> Abs_CSPF (\<lambda> sb. (sbDom\<cdot>sb = (spfDom\<cdot>f - ran(m)) \<union> dom(m)) \<leadsto> (f \<rightleftharpoons> (sbRenameChMap sb m)))" 
+  
+definition spfFeedbackOperator_new :: "'a SPF \<Rightarrow> (channel \<rightharpoonup> channel) \<Rightarrow> 'a SPF" where
+"spfFeedbackOperator_new f m \<equiv> spfFeedbackOperator (spfRename f m)"   
+
+definition map_injective :: "(channel \<rightharpoonup> channel) \<Rightarrow> bool" where
+"map_injective m \<longleftrightarrow> (\<forall> x \<in> dom(m). \<forall> y \<in> dom(m). m x = m y \<longrightarrow> x = y)"
+
+definition rename_map_well :: "'m SB \<Rightarrow> (channel \<rightharpoonup> channel) \<Rightarrow> bool" where
+"rename_map_well sb m \<longleftrightarrow> map_injective m \<and> (dom(m) \<subseteq> sbDom\<cdot>sb)"
+  
+subsection \<open>map_inverse\<close>
+  
+  
+
+
+  
+subsection \<open>sbRenameChMap\<close>
+  
+ 
+lemma t10: assumes "map_injective m" 
+  shows "sb_well (\<lambda>c. if (c \<in> (sbDom\<cdot>sb \<inter> dom(m) - ran(m))) then None else Rep_SB(sb)((mapIdFunct (map_inverse m))(c)))" 
+  sorry
+    
+lemma t13: assumes "map_injective m" 
+  shows "sb_well (\<lambda>c. if (c \<in> sbDom\<cdot>sb \<and> c \<in> dom m \<and> c \<notin> ran m) then None else Rep_SB(sb)((mapIdFunct (map_inverse m))(c)))" 
+  sorry
+
+lemma t11: assumes "map_injective m" and "c \<notin> ran(m)" shows "(mapIdFunct (map_inverse m) c) = c"
+  apply(simp add: mapIdFunct_def map_inverse_def)
+  by (simp add: assms)
+    
+lemma t12: assumes "map_injective m" and "(m ch1) = Some ch2" shows "(mapIdFunct (map_inverse m) ch2) = ch1"
+proof - 
+  have f1: "ch2 \<in> ran m"
+    by (meson assms ranI)
+  show ?thesis
+    using f1 apply(simp add: mapIdFunct_def map_inverse_def)
+    proof -
+      have "\<And>c. \<not> map_injective m \<or> ch1 \<notin> dom m \<or> c \<notin> dom m \<or> m c \<noteq> Some ch2 \<or> c = ch1"
+        by (metis assms(2) map_injective_def)
+      then have f1: "\<And>c. ch1 \<notin> dom m \<or> c \<notin> dom m \<or> m c \<noteq> Some ch2 \<or> c = ch1"
+        by (metis assms(1))
+      obtain cc :: "(channel \<Rightarrow> bool) \<Rightarrow> channel \<Rightarrow> channel" where
+        f2: "\<And>p c. (\<not> p c \<or> p (cc p c) \<or> The p = c) \<and> (\<not> p c \<or> cc p c \<noteq> c \<or> The p = c)"
+        by (metis (no_types) the_equality)
+      then have "\<And>c. m c \<noteq> Some ch2 \<or> ch1 \<notin> dom m \<or> cc (\<lambda>c. m c = Some ch2) c \<notin> dom m \<or> (THE c. m c = Some ch2) = c \<or> cc (\<lambda>c. m c = Some ch2) c = ch1"
+        using f1 by meson
+      then have "\<And>c. m c \<noteq> Some ch2 \<or> ch1 \<notin> dom m \<or> m (cc (\<lambda>c. m c = Some ch2) c) = None \<or> (THE c. m c = Some ch2) = c \<or> cc (\<lambda>c. m c = Some ch2) c = ch1"
+        by (simp add: domIff)
+      then have "\<And>c. m c \<noteq> Some ch2 \<or> ch1 \<notin> dom m \<or> Some ch2 = None \<or> (THE c. m c = Some ch2) = c \<or> cc (\<lambda>c. m c = Some ch2) c = ch1"
+        using f2 by (metis (mono_tags, lifting))
+      then have f3: "\<And>c. m c \<noteq> Some ch2 \<or> ch1 \<notin> dom m \<or> (THE c. m c = Some ch2) = c \<or> cc (\<lambda>c. m c = Some ch2) c = ch1"
+        by (simp add: option.distinct(1))
+      have "m ch1 = Some ch2 \<and> ch1 \<in> dom m \<and> (THE c. m c = Some ch2) \<noteq> ch1 \<or> (THE c. m c = Some ch2) = ch1"
+        by (simp add: assms(2) domIff)
+      then show "(THE c. m c = Some ch2) = ch1"
+        using f3 f2 by meson
+    qed
+qed
+    
+lemma sbRenameChMap_getCh: assumes "(m ch1) = Some ch2" and "map_injective m" shows "(sbRenameChMap sb m) . ch2 = sb . ch1"
+proof - 
+  have f1: "ch2 \<in> ran m"
+    by (meson assms ranI)
+  have f2: " Rep_SB sb \<rightharpoonup> ch1 = sb . ch1"
+    by (simp add: sbGetCh_def)
+  have f3: "(THE z. (m z = Some ch2)) = ch1"
+    proof -
+      have f1: "\<And>c. ch1 \<notin> dom m \<or> c \<notin> dom m \<or> m c \<noteq> Some ch2 \<or> c = ch1"
+        by (metis assms(1) assms(2) map_injective_def)
+      have f2: "ch1 \<in> dom m"
+        using assms(1) by blast
+      obtain cc :: "(channel \<Rightarrow> bool) \<Rightarrow> channel \<Rightarrow> channel" where
+        f3: "\<And>p c. (\<not> p c \<or> p (cc p c) \<or> The p = c) \<and> (\<not> p c \<or> cc p c \<noteq> c \<or> The p = c)"
+        by (metis (no_types) the_equality)
+      then have "\<And>c. m c \<noteq> Some ch2 \<or> ch1 \<notin> dom m \<or> cc (\<lambda>c. m c = Some ch2) c \<notin> dom m \<or> (THE c. m c = Some ch2) = c \<or> cc (\<lambda>c. m c = Some ch2) c = ch1"
+        using f1 by meson
+      then have "\<And>c. m c \<noteq> Some ch2 \<or> ch1 \<notin> dom m \<or> m (cc (\<lambda>c. m c = Some ch2) c) = None \<or> (THE c. m c = Some ch2) = c \<or> cc (\<lambda>c. m c = Some ch2) c = ch1"
+        by blast
+      then have "\<And>c. m c \<noteq> Some ch2 \<or> ch1 \<notin> dom m \<or> Some ch2 = None \<or> (THE c. m c = Some ch2) = c \<or> cc (\<lambda>c. m c = Some ch2) c = ch1"
+        using f3 by (metis (mono_tags, lifting))
+      then have "\<And>c. m c \<noteq> Some ch2 \<or> ch1 \<notin> dom m \<or> (THE c. m c = Some ch2) = c \<or> cc (\<lambda>c. m c = Some ch2) c = ch1"
+        by blast
+      then show ?thesis
+        using f3 f2 by (meson assms(1))
+    qed
+  show ?thesis  
+    apply(simp only: sbRenameChMap_def)
+    apply(simp add: sbGetCh_def)
+    apply(subst rep_abs)
+    apply(simp add: t13 assms)
+    apply(simp add: mapIdFunct_def map_inverse_def f1)
+    by(simp add: f3 f2)
+qed
+    
+lemma sbRenameChMap_getCh2: assumes "\<not>(\<exists> ch2. ((m ch2) = Some ch1))" and "ch1 \<notin> (sbDom\<cdot>sb \<inter> dom(m) - ran(m))" and "map_injective m" 
+                            shows "(sbRenameChMap sb m) . ch1 = sb . ch1" 
+proof - 
+  have f1: "ch1 \<notin> ran m"
+    by (meson assms ran2exists)
+  have f2: " Rep_SB sb \<rightharpoonup> ch1 = sb . ch1"
+    by (simp add: sbGetCh_def)
+  have f3: "(ch1 \<in> sbDom\<cdot>sb \<and> ch1 \<in> dom m \<and> ch1 \<notin> ran m) = False"
+    using assms(2) by auto
+  show ?thesis  
+    apply(simp add: sbRenameChMap_def)
+    apply(subst sbGetCh_def, simp)
+    apply(subst rep_abs)
+     apply(simp add: t13 assms)
+      apply(simp add: f3)
+    apply(simp add: mapIdFunct_def map_inverse_def f1)
+    by(simp add: f2)
+qed  
+
+lemma sbRenameChMap_sbDom: assumes "rename_map_well sb m" shows "sbDom\<cdot>(sbRenameChMap sb m) = (sbDom\<cdot>sb - dom(m)) \<union> ran(m)"
+proof - 
+  have f0: "map_injective m"
+    using assms rename_map_well_def by auto
+  have f11: "\<And>x. (x \<in> ran m \<longrightarrow> (THE z. m z = Some x) \<in> dom(m))"
+    using f0 mapIdFunct_def map_inverse_def ran2exists t12 by fastforce
+  have f12: "\<And>x. (x \<in> ran m \<longrightarrow> (THE z. m z = Some x) \<in> sbDom\<cdot>sb)"
+    using assms f11 rename_map_well_def by blast
+  have f1: "\<And>x. (x \<in> ran m \<longrightarrow> (\<exists>y. Rep_SB sb (THE z. m z = Some x) = Some y))"
+    by (metis f12 sbgetchE)
+  have f21: "\<And>x. (x \<in> dom m \<longrightarrow> x \<in> sbDom\<cdot>sb)"
+    using assms rename_map_well_def by auto
+  have f2: "\<And>x. (x \<notin> ran m \<longrightarrow> (x \<in> dom m \<longrightarrow> x \<notin> sbDom\<cdot>sb) \<longrightarrow> (\<exists>y. Rep_SB sb x = Some y) = (x \<in> sbDom\<cdot>sb \<and> x \<notin> dom m))"
+    apply(simp add: f21)
+    using sbdom_insert by fastforce
+  show ?thesis
+    apply(simp add: sbRenameChMap_def)
+    apply(subst sbDom_def, simp add: t10)
+    apply(subst rep_abs)
+    apply(simp add: t13 f0 map_inverse_def)
+    apply(simp only: mapIdFunct_def f0 map_inverse_def)
+    apply(subst dom_def)
+    apply(subst set_eqI)
+    apply(simp_all)
+     using f1 f2 by auto 
+qed
+  
+  
+subsection \<open>spfRename\<close>
+
+  
+lemma spfRename_cont: "cont (\<lambda> sb. (sbDom\<cdot>sb = (spfDom\<cdot>f - ran(m)) \<union> dom(m)) \<leadsto> (f \<rightleftharpoons> (sbRenameChMap sb m)))"
+  sorry
+    
+lemma spfRename_spf_well: "spf_well (\<Lambda> sb. (sbDom\<cdot>sb = (spfDom\<cdot>f - ran(m)) \<union> dom(m)) \<leadsto> (f \<rightleftharpoons> (sbRenameChMap sb m)))"
+  apply(simp add: spf_well_def spfRename_cont)
+  apply(simp only: domIff2)
+  apply(simp add: sbdom_rep_eq)
+  sorry
+    
+lemma spfRename_RepAbs: "Rep_CSPF (Abs_CSPF (\<lambda> sb. (sbDom\<cdot>sb = (spfDom\<cdot>f - ran(m)) \<union> dom(m)) \<leadsto> (f \<rightleftharpoons> (sbRenameChMap sb m)))) = 
+  (\<lambda> sb. (sbDom\<cdot>sb = (spfDom\<cdot>f - ran(m)) \<union> dom(m)) \<leadsto> (f \<rightleftharpoons> (sbRenameChMap sb m)))"
+  by(simp add: spfRename_cont spfRename_spf_well)
+    
+lemma spfRename_spfDom: "spfDom\<cdot>(spfRename f m) = (spfDom\<cdot>f - ran(m)) \<union> dom(m)"
+  apply(simp add: spfRename_def)
+  apply(subst spfDomAbs)
+    by (simp_all add: spfRename_cont spfRename_spf_well)
+
+lemma spfRename_spfRan: "spfRan\<cdot>(spfRename f m) = spfRan\<cdot>f"
+  sorry  
+
+    
+subsection \<open>spfFeedbackOperator_new\<close>
+  
+  
+lemma spfFeedbackOperator_new_spfDom: "spfDom\<cdot>(spfFeedbackOperator_new f m) = (spfDom\<cdot>f - ran(m)) \<union> dom(m)"
+  apply(simp add: spfFeedbackOperator_new_def)
+  apply(simp add: spfRename_spfDom spfRename_spfRan)
+  sorry
+
+lemma spfFeedbackOperator_new_spfRan: "spfRan\<cdot>(spfFeedbackOperator_new f m) = spfRan\<cdot>f"
+  sorry   
+  
+  
+section \<open>General lemmas parcomp and sercomp\<close>  
 
   
 (* Should already be proven somewhere*)  
 lemma parcomp_cont[simp]: "cont (\<lambda> x. (sbDom\<cdot>x = spfDom\<cdot>f1 \<union> spfDom\<cdot>f2 ) \<leadsto> ((f1 \<rightleftharpoons> (x \<bar>spfDom\<cdot>f1)) \<uplus> (f2 \<rightleftharpoons> (x\<bar>spfDom\<cdot>f2))))"
-sorry  
+  sorry  
   
 lemma parcomp_spf_well[simp]: "spf_well (\<Lambda> x. (sbDom\<cdot>x = spfDom\<cdot>f1 \<union> spfDom\<cdot>f2 ) \<leadsto> ((f1 \<rightleftharpoons> (x \<bar>spfDom\<cdot>f1)) \<uplus> (f2 \<rightleftharpoons> (x\<bar>spfDom\<cdot>f2))))"  
-sorry
+  apply(simp add: spf_well_def)
+  apply(simp only: domIff2)
+  apply(simp add: sbdom_rep_eq)
+  by(auto) 
 
 lemma sercomp_cont[simp]: "cont (\<lambda> x. (sbDom\<cdot>x =  spfDom\<cdot>f1) \<leadsto> ((f1 \<rightleftharpoons> x) \<uplus> (f2 \<rightleftharpoons> (f1 \<rightleftharpoons> x))))"
-sorry  
+  sorry  
   
 lemma sercomp_spf_well[simp]: "spf_well (\<Lambda> x. (sbDom\<cdot>x =  spfDom\<cdot>f1) \<leadsto> ((f1 \<rightleftharpoons> x) \<uplus> (f2 \<rightleftharpoons> (f1 \<rightleftharpoons> x))))"  
-sorry  
+  sorry
 
 lemma parcomp_repAbs: "Rep_CSPF (Abs_CSPF (\<lambda> x. (sbDom\<cdot>x = spfDom\<cdot>f1 \<union> spfDom\<cdot>f2 ) \<leadsto> ((f1 \<rightleftharpoons> (x \<bar>spfDom\<cdot>f1)) \<uplus> (f2 \<rightleftharpoons> (x\<bar>spfDom\<cdot>f2))))) 
                       = (\<lambda> x. (sbDom\<cdot>x = spfDom\<cdot>f1 \<union> spfDom\<cdot>f2 ) \<leadsto> ((f1 \<rightleftharpoons> (x \<bar>spfDom\<cdot>f1)) \<uplus> (f2 \<rightleftharpoons> (x\<bar>spfDom\<cdot>f2))))"
@@ -26,87 +222,10 @@ lemma parcomp_repAbs: "Rep_CSPF (Abs_CSPF (\<lambda> x. (sbDom\<cdot>x = spfDom\
 lemma sercomp_repAbs: "Rep_CSPF (Abs_CSPF (\<lambda> x. (sbDom\<cdot>x =  spfDom\<cdot>f1) \<leadsto> ((f1 \<rightleftharpoons> x) \<uplus> (f2 \<rightleftharpoons> (f1 \<rightleftharpoons> x))))) 
                       = (\<lambda> x. (sbDom\<cdot>x =  spfDom\<cdot>f1) \<leadsto> ((f1 \<rightleftharpoons> x) \<uplus> (f2 \<rightleftharpoons> (f1 \<rightleftharpoons> x))))"
   by simp
+    
   
-section \<open> Feedback Definitions \<close>  
+section \<open>SPF Definitions\<close>
 
-  
-definition MapIdFunct :: "(channel \<rightharpoonup> channel) \<Rightarrow> channel \<Rightarrow> channel" where
-"MapIdFunct m \<equiv> (\<lambda> c. case m c of None \<Rightarrow> c | Some y \<Rightarrow> y )" 
-
-definition the_inv_into :: "'a set \<Rightarrow> ('a \<Rightarrow> 'b) \<Rightarrow> ('b \<Rightarrow> 'a)"
-  where "the_inv_into A f = (\<lambda>x. THE y. y \<in> A \<and> f y = x)"
-    
-definition map_inverse :: "(channel \<rightharpoonup> channel) \<Rightarrow> (channel \<rightharpoonup> channel)" where
-"map_inverse m \<equiv> (\<lambda>x. if (x \<in> (ran m)) then Some ((\<lambda> y. (THE z. m z = Some y)) x) else None)"
-    
-definition sbRenameChMap :: "'m SB \<Rightarrow> (channel \<rightharpoonup> channel) \<Rightarrow> 'm SB" where
-"sbRenameChMap sb m \<equiv> Abs_SB (\<lambda>c. Rep_SB(sb)((MapIdFunct (map_inverse m))(c)))"  
-  
-definition spfRename :: "'a SPF \<Rightarrow> (channel \<rightharpoonup> channel) \<Rightarrow> 'a SPF" where
-"spfRename f m \<equiv> Abs_CSPF (\<lambda> sb. (sbDom\<cdot>sb = (spfDom\<cdot>f - ran(m)) \<union> dom(m)) \<leadsto> (f \<rightleftharpoons> (sbRenameChMap sb m)))" 
-  
-definition spfFeedbackOperator_new :: "'a SPF \<Rightarrow> (channel \<rightharpoonup> channel) \<Rightarrow> 'a SPF" where
-"spfFeedbackOperator_new f m \<equiv> spfFeedbackOperator (spfRename f m)"   
-
-subsection \<open> cont, spf_well, rename lemmas \<close>
-
-lemma spfRename_spfDom: "spfDom\<cdot>(spfRename f m) = (spfDom\<cdot>f - ran(m)) \<union> dom(m)"
-  sorry
-    
-lemma spfRename_spfRan: "spfRan\<cdot>(spfRename f m) = spfRan\<cdot>f"
-  sorry    
-
-lemma spfRename_cont: "cont (\<lambda> sb. (sbDom\<cdot>sb = (spfDom\<cdot>f - ran(m)) \<union> dom(m)) \<leadsto> (f \<rightleftharpoons> (sbRenameChMap sb m)))"
-  sorry
-    
-lemma spfRename_spf_well: "spf_well (\<Lambda> sb. (sbDom\<cdot>sb = (spfDom\<cdot>f - ran(m)) \<union> dom(m)) \<leadsto> (f \<rightleftharpoons> (sbRenameChMap sb m)))"
-  sorry
-    
-lemma spfRename_RepAbs: "Rep_CSPF (Abs_CSPF (\<lambda> sb. (sbDom\<cdot>sb = (spfDom\<cdot>f - ran(m)) \<union> dom(m)) \<leadsto> (f \<rightleftharpoons> (sbRenameChMap sb m)))) = 
-  (\<lambda> sb. (sbDom\<cdot>sb = (spfDom\<cdot>f - ran(m)) \<union> dom(m)) \<leadsto> (f \<rightleftharpoons> (sbRenameChMap sb m)))"
-  by(simp add: spfRename_cont spfRename_spf_well)
-
-subsection \<open>rename lemmas \<close> 
-  
-(* to solve this lemmata it may be neccessary to redefine sbRenameChMap*)
-  
-lemma sbRenameChMap_sbDom: "sbDom\<cdot>(sbRenameChMap sb m) = (sbDom\<cdot>sb - dom(m)) \<union> ran(m)" 
-  sorry
- 
-lemma t10: "sb_well (\<lambda>c. Rep_SB(sb)((MapIdFunct (map_inverse m))(c)))"    
-  sorry
-  
-lemma sbRenameChMap_getCh: assumes "(m ch1) = Some ch2" and "\<not>(\<exists> ch3. ((m ch3) = Some ch2))" shows "(sbRenameChMap sb m) . ch2 = sb . ch1"
-proof - 
-  have f1: "ch2 \<in> ran m"
-    by (meson assms ranI)
-  have f2: " Rep_SB sb \<rightharpoonup> ch1 = sb . ch1"
-    by (simp add: sbGetCh_def)
-  have f3: "(THE z. (m z = Some ch2)) = ch1"
-    using assms(1) assms(2) by auto
-  show ?thesis  
-    apply(simp add: sbRenameChMap_def)
-    apply(subst sbGetCh_def, simp)
-    apply(subst rep_abs, simp add: t10)
-    apply(simp add: MapIdFunct_def map_inverse_def f1)
-    by(simp add: f3 f2)
-qed
-    
-lemma sbRenameChMap_getCh2: assumes "\<not>(\<exists> ch2. ((m ch2) = Some ch1))"  shows "(sbRenameChMap sb m) . ch1 = sb . ch1" 
-proof - 
-  have f1: "ch1 \<notin> ran m"
-    by (meson assms ran2exists)
-  have f2: " Rep_SB sb \<rightharpoonup> ch1 = sb . ch1"
-    by (simp add: sbGetCh_def)
-  show ?thesis  
-    apply(simp add: sbRenameChMap_def)
-    apply(subst sbGetCh_def, simp)
-    apply(subst rep_abs, simp add: t10)
-    apply(simp add: MapIdFunct_def map_inverse_def f1)
-    by(simp add: f2)
-qed
-    
-section \<open> SPF Definitions \<close>
   
 definition idC :: "nat SPF" where
 "idC \<equiv> SPF1x1 sb_id (c1, c3)"
@@ -118,16 +237,20 @@ definition addC :: "nat SPF" where
 "addC \<equiv> SPF2x1 add (c3, c4, c5)" 
 
 abbreviation innerSum4SPF :: "nat SPF" where
-  "innerSum4SPF \<equiv> ((idC \<parallel> append0C) \<circ> addC)"
+"innerSum4SPF \<equiv> ((idC \<parallel> append0C) \<circ> addC)"
 
 definition sum4SPF :: "nat SPF" where
 "sum4SPF \<equiv> spfFeedbackOperator_new ((idC \<parallel> append0C) \<circ> addC) [c5 \<mapsto> c2]"
 
 abbreviation innerFeedbackSum4SPF :: "nat SPF" where
-"innerFeedbackSum4SPF \<equiv> (spfRename innerSum4SPF [c5 \<mapsto> c2])"
+"innerFeedbackSum4SPF \<equiv> (spfRename innerSum4SPF [c5 \<mapsto> c2])"  
+  
+  
+subsection \<open>Requirements\<close>
 
-subsection \<open> requirements \<close>
+subsubsection \<open>spfDom, spfRan\<close>
 
+  
 lemma [simp]: "spfDom\<cdot>idC = {c1}"
   by(auto simp add: idC_def SPF1x1_dom)
     
@@ -144,8 +267,12 @@ lemma [simp]: "spfDom\<cdot>addC = {c3, c4}"
   by(auto simp add: addC_def SPF1x1_dom)
     
 lemma [simp]: "spfRan\<cdot>addC = {c5}"
-  by(auto simp add: addC_def SPF1x1_ran)    
-    
+  by(auto simp add: addC_def SPF1x1_ran)   
+  
+  
+subsubsection \<open>Composition par\<close>
+
+  
 lemma [simp]: "I idC append0C = {c1, c2}"
 by (auto simp add: I_def)
 
@@ -153,10 +280,14 @@ lemma [simp]: "Oc idC append0C = {c3, c4}"
 by (auto simp add: Oc_def)
 
 lemma [simp]: "L idC append0C = {}"
-by (auto simp add: L_def)
+by (auto simp add: L_def)  
 
 lemma [simp]: "spfComp_well idC append0C"
-by (simp add: spfComp_well_def)  
+  by (simp add: spfComp_well_def) 
+    
+
+subsubsection \<open>spfDom, spfRan\<close>
+  
   
 lemma domIdAppend[simp]: "spfDom\<cdot>(idC \<parallel> append0C) = {c1, c2}"
 apply(subst parCompDom, simp_all)
@@ -166,8 +297,12 @@ by simp_all
 lemma ranIdAppend[simp]: "spfRan\<cdot>(idC \<parallel> append0C) = {c3, c4}"
 apply(subst parCompRan, simp_all)
 apply(subst spfComp_ran_Oc)
-by simp_all  
-
+by simp_all    
+  
+    
+subsubsection \<open>Composition ser\<close>
+  
+  
 lemma [simp]: "I (idC \<parallel> append0C) addC = {c1, c2}"
   by(simp add: I_def)
     
@@ -178,7 +313,11 @@ lemma [simp]: "L (idC \<parallel> append0C) addC = {c3, c4}"
   by(auto simp add: L_def) 
     
 lemma [simp]: "pL (idC \<parallel> append0C) addC = {}"
-  by(auto simp add: pL_def) 
+  by(auto simp add: pL_def)   
+  
+    
+subsubsection \<open>Feedback\<close>
+  
   
 lemma domInnerSum4SPF[simp]: "spfDom\<cdot>(innerSum4SPF) = {c1, c2}"
   sorry
@@ -187,23 +326,33 @@ lemma ranInnerSum4SPF[simp]: "spfRan\<cdot>(innerSum4SPF) = {c3, c4, c5}"
   sorry 
 
 lemma domInnerFeedbackSum4SPF: "spfDom\<cdot>(innerFeedbackSum4SPF) = {c1, c5}"
-  sorry   
+proof -
+  have f1: "\<And>z c s. z = None \<or> insert c (spfDom\<cdot>(s::nat SPF) - ran (Map.empty(c := z))) = spfDom\<cdot>(spfRename s (Map.empty(c := z)))"
+    by (simp add: spfRename_spfDom sup_bot.right_neutral)
+  have "c2 \<notin> {c1}"
+    by blast
+  then have "insert c5 ({c1, c2} - {c2}) = {c1, c5}"
+    by fastforce
+  then show ?thesis
+    using f1 by (metis domInnerSum4SPF option.simps(3) ran_empty ran_map_upd)
+qed
+  
 
-lemma ranInnerFeedbackSum4SPF: "spfRan\<cdot>(innerFeedbackSum4SPF) = {c5}"
-  sorry
+lemma ranInnerFeedbackSum4SPF: "spfRan\<cdot>(innerFeedbackSum4SPF) = {c3, c4, c5}"
+  by (simp add: spfRename_spfRan)
     
-lemma ranInnerFeedbackSum4SPF_sb: assumes "sbDom\<cdot>sb = {c5}" shows "sbDom\<cdot>(innerFeedbackSum4SPF\<rightleftharpoons>sb) = spfRan\<cdot>(innerFeedbackSum4SPF)"
+lemma ranInnerFeedbackSum4SPF_sb: assumes "sbDom\<cdot>sb = {c1, c5}" shows "sbDom\<cdot>(innerFeedbackSum4SPF\<rightleftharpoons>sb) = spfRan\<cdot>(innerFeedbackSum4SPF)"
   sorry
   
 lemma [simp]: "spfDom\<cdot>sum4SPF = {c1}"
-sorry  
+  sorry  
 
-lemma [simp]: "spfDom\<cdot>sum4SPF = {c3, c4, c5}"
-sorry      
-
+lemma [simp]: "spfRan\<cdot>sum4SPF = {c3, c4, c5}"
+  sorry  
   
-subsection \<open> apply lemmas \<close>    
-
+  
+subsubsection \<open>Apply lemmas\<close>
+  
   
 lemma innerSum4SPF_c5_eq: assumes "sbDom\<cdot>sb = I (idC \<parallel> append0C) addC" shows "(innerSum4SPF \<rightleftharpoons> sb) . c5 = add\<cdot>(sb . c1)\<cdot>(\<up>0\<bullet>(sb . c2))"
 proof - 
@@ -239,131 +388,180 @@ proof -
     by(simp add: sb_id_def appendElem2_def)
 qed  
   
-lemma innerFeedbackSum4SPF_c5_eq: assumes "sbDom\<cdot>sb = {c1}" and "sbDom\<cdot>z = {c5}" shows
+lemma innerFeedbackSum4SPF_c5_eq: assumes "sbDom\<cdot>sb = {c1}" and "c5 \<in> sbDom\<cdot>z" shows
     "(innerFeedbackSum4SPF \<rightleftharpoons> ((sb \<uplus> z)\<bar> {c1, c5})) . c5 = add\<cdot>(sb . c1)\<cdot>(\<up>0\<bullet>(z . c5))"
 proof - 
+  have f0: "insert c5 ({c1, c2} - {c2}) = {c1, c5}"
+    by auto
   have f1: "(sbRenameChMap ((sb \<uplus> z)\<bar>{c1, c5}) [c5 \<mapsto> c2]) . c1 = sb . c1"
-    apply(simp add: assms)
+    sorry
+    (*apply(simp add: assms)
     apply(subst sbRenameChMap_getCh2)
-    by(simp_all add: assms)
+    by(simp_all add: assms map_injective_def)*)
   have f2: "(sbRenameChMap ((sb \<uplus> z)\<bar>{c1, c5}) [c5 \<mapsto> c2]) . c2 = z . c5"
-    apply(simp add: assms)
+    sorry
+    (*apply(simp add: assms)
     apply(subst sbRenameChMap_getCh)
-      apply(simp)
-      apply (metis channel.distinct(61) ranInnerFeedbackSum4SPF ranInnerSum4SPF singleton_insert_inj_eq' spfRename_spfRan)
-    by (simp add: assms(2))
+    apply(simp)
+    by (simp_all add: assms(2) map_injective_def)*)
   have f3: "sbDom\<cdot>(sbRenameChMap ((sb \<uplus> z)\<bar>{c1, c5}) [c5 \<mapsto> c2]) = I (idC\<parallel>append0C) addC"
     apply(simp add: assms)
-    apply(simp add: sbRenameChMap_sbDom assms)
+    apply(subst sbRenameChMap_sbDom)
+     apply(simp_all add: rename_map_well_def map_injective_def assms)
     by auto
   show ?thesis 
   apply(simp only: spfRename_def)
   apply(subst spfRename_RepAbs) 
     apply(simp add: assms)
     apply(subst innerSum4SPF_c5_eq)
-     apply(simp add: f3)
-    apply(subst f1)
-    apply(subst f2)
+     apply (metis (no_types, lifting) Diff_insert_absorb channel.distinct(1) f3 insert_absorb insert_commute singleton_insert_inj_eq')
+    apply(subst f0, subst f0, subst f0) (* why? *)
+    apply(subst f1, subst f2)
       by auto
-qed
+qed  
+
+lemma innerFeedbackSum4SPF_c3_eq: assumes "sbDom\<cdot>sb = {c1}" and "c5 \<in> sbDom\<cdot>z" shows
+    "(innerFeedbackSum4SPF \<rightleftharpoons> ((sb \<uplus> z)\<bar> {c1, c5})) . c3 = sb . c1"
+  sorry
     
+lemma innerFeedbackSum4SPF_c4_eq: assumes "sbDom\<cdot>sb = {c1}" and "c5 \<in> sbDom\<cdot>z" shows
+    "(innerFeedbackSum4SPF \<rightleftharpoons> ((sb \<uplus> z)\<bar> {c1, c5})) . c4 = (appendElem2 0\<cdot>(z . c5))"
+ sorry    
   
-section \<open> eq proof \<close>
+  
+section \<open>Equality proof\<close>
 
-  
-lemma t5: assumes "sbDom\<cdot>sb = {c1}" shows 
+(* requirements *)
+
+lemma t6: assumes "sbDom\<cdot>sb = {c1}" shows 
     "cont (\<lambda> z. (innerFeedbackSum4SPF\<rightleftharpoons>((sb \<uplus> z)\<bar> {c1, c5})))"
-  by (metis domInnerFeedbackSum4SPF spfFeedH_cont)
+  by (metis domInnerFeedbackSum4SPF spfFeedH_cont)  
 
-lemma t4: assumes "sbDom\<cdot>sb = {c1}" and "sbDom\<cdot>x = {c5} " shows
-    "(\<Lambda> z. (innerFeedbackSum4SPF\<rightleftharpoons>((sb \<uplus> z)\<bar> {c1, c5})))\<cdot>x = (\<Lambda> z. [c5 \<mapsto> add\<cdot>(sb . c1)\<cdot>(appendElem2 0\<cdot>(z . c5))]\<Omega>)\<cdot>x" 
-proof - 
-  have f1: "sbDom\<cdot>(innerFeedbackSum4SPF\<rightleftharpoons>(sb \<uplus> x)) = {c5}"
-    by (metis channel.distinct(61) ranInnerFeedbackSum4SPF ranInnerSum4SPF singleton_insert_inj_eq' spfRename_spfRan)
-  have f2: "sbDom\<cdot>([c5 \<mapsto> add\<cdot>(sb . c1)\<cdot>(appendElem2 0\<cdot>(x . c5))]\<Omega>) = {c5}"
-    by(simp add: sbdom_rep_eq)
-  have f3: "innerFeedbackSum4SPF\<rightleftharpoons>(sb \<uplus> x) = innerFeedbackSum4SPF\<rightleftharpoons>((sb \<uplus> x)\<bar> {c1, c5})"
-    by (simp add: assms(1) assms(2))
-  show ?thesis  
-    apply(simp add: assms)
-    apply(subst Abs_cfun_inverse2)
-     apply(subst t5)
-      apply(simp_all add: assms)
-    apply(subst sb_eq, simp_all)
-     apply(simp add: f1 f2)
-    apply(simp add: f1)
-    apply(subst f3)
-    apply(subst innerFeedbackSum4SPF_c5_eq)
-      by(simp_all add: assms appendElem2_def)
-qed
+lemma t7: assumes "sbDom\<cdot>sb = {c1}" shows 
+    "cont (\<lambda> z. [c3 \<mapsto> (sb . c1), c4 \<mapsto> (appendElem2 0\<cdot>(z . c5)), c5 \<mapsto> add\<cdot>(sb . c1)\<cdot>(appendElem2 0\<cdot>(z . c5))]\<Omega>)"
+  sorry    
+    
+lemma t5: "c5 \<in> sbDom\<cdot>(iterate i\<cdot>(\<Lambda> z. innerFeedbackSum4SPF\<rightleftharpoons>((sb \<uplus> z)\<bar>{c1, c5}))\<cdot>({c3, c4, c5}^\<bottom>))"  
+  sorry
   
-lemma sbDomSB_eq: assumes "sbDom\<cdot>sb = {ch1}" shows "sb = ([ch1 \<mapsto> sb . ch1]\<Omega>)"
-  apply(subst sb_eq, simp_all)
-   apply (metis Rep_SB_inverse assms dom_eq_singleton_conv fun_upd_same insertI1 sbdom_insert sbgetchE)
-    by (metis Rep_SB_inverse assms dom_eq_singleton_conv fun_upd_same sbdom_insert sbgetchE singletonD)
+lemma t4: assumes "sbDom\<cdot>sb = {c1}" and "c5 \<in> sbDom\<cdot>x" shows
+    "((\<Lambda> z. (innerFeedbackSum4SPF\<rightleftharpoons>((sb \<uplus> z)\<bar> {c1, c5})))\<cdot>x)= 
+     ((\<Lambda> z. [c3 \<mapsto> (sb . c1), c4 \<mapsto> (appendElem2 0\<cdot>(z . c5)), c5 \<mapsto> add\<cdot>(sb . c1)\<cdot>(appendElem2 0\<cdot>(z . c5))]\<Omega>)\<cdot>x)"
+proof - 
+  have f1: "sbDom\<cdot>(innerFeedbackSum4SPF\<rightleftharpoons>((sb \<uplus> x)\<bar>{c1, c5})) = {c3, c4, c5}"
+    sorry
+  have f2: "sbDom\<cdot>([c3 \<mapsto> (sb . c1), c4 \<mapsto> (appendElem2 0\<cdot>(x . c5)), c5 \<mapsto> add\<cdot>(sb . c1)\<cdot>(appendElem2 0\<cdot>(x . c5))]\<Omega>) = {c3, c4, c5}"
+    by(auto simp add: sbdom_rep_eq)
+  show ?thesis
+    apply(subst Abs_cfun_inverse2)
+    apply(subst t6, simp add: assms, simp)
+    apply(subst Abs_cfun_inverse2)
+     apply(subst t7, simp add: assms, simp)
+    apply(subst sb_eq, simp_all)
+    apply(simp_all add: f1 f2)
+    apply(case_tac c)
+    apply(simp_all)
+     apply(subst innerFeedbackSum4SPF_c3_eq, simp_all add: assms)
+     apply(simp add: sbgetch_rep_eq)
+      apply(subst innerFeedbackSum4SPF_c4_eq, simp_all add: assms)
+      apply(simp add: sbgetch_rep_eq)
+      apply(subst innerFeedbackSum4SPF_c5_eq, simp_all add: assms)
+      apply(simp add: sbgetch_rep_eq)
+    sorry
+qed
 
+lemma t8: assumes "sbDom\<cdot>sb = {c1}" shows 
+        "sbfun_io_eq (\<Lambda> z. [c3 \<mapsto> (sb . c1), c4 \<mapsto> (appendElem2 0\<cdot>(z . c5)), c5 \<mapsto> add\<cdot>(sb . c1)\<cdot>(appendElem2 0\<cdot>(z . c5))]\<Omega>) {c3, c4, c5}"
+    apply(subst Abs_cfun_inverse2)
+     apply(subst t7, simp_all add: assms)
+    apply(simp add: sbdom_rep_eq)
+  by auto
+    
+lemma t22: "([c3 \<mapsto> sb . c1, c4 \<mapsto> appendElem2 0\<cdot>(z . c5), c5 \<mapsto> add\<cdot>(sb . c1)\<cdot>(appendElem2 0\<cdot>(z . c5))]\<Omega>) . c5 = 
+            add\<cdot>(sb . c1)\<cdot>(appendElem2 0\<cdot>(z . c5))"    
+  by (simp add: sbgetch_rep_eq)
+
+(* iterate eq lemmas *)  
+  
 lemma t2: assumes "sbDom\<cdot>sb = {c1}" shows
-  "iterate i\<cdot>(\<Lambda> z. (innerFeedbackSum4SPF\<rightleftharpoons>((sb \<uplus> z)\<bar> {c1, c5})))\<cdot>({c5}^\<bottom>) =  
-   iterate i\<cdot>(\<Lambda> z. [c5 \<mapsto> add\<cdot>(sb . c1)\<cdot>(appendElem2 0\<cdot>(z . c5))]\<Omega>)\<cdot>({c5}^\<bottom>)"
+  "(iterate i\<cdot>(\<Lambda> z. (innerFeedbackSum4SPF\<rightleftharpoons>((sb \<uplus> z)\<bar> {c1, c5})))\<cdot>({c3, c4, c5}^\<bottom>)) =  
+   (iterate i\<cdot>(\<Lambda> z. [c3 \<mapsto> (sb . c1), c4 \<mapsto> (appendElem2 0\<cdot>(z . c5)), c5 \<mapsto> add\<cdot>(sb . c1)\<cdot>(appendElem2 0\<cdot>(z . c5))]\<Omega>)\<cdot>({c3, c4, c5}^\<bottom>))"
 proof (induction i)
   case 0
   then show ?case 
     by(simp add: iterate_def)
-next
   case (Suc i)
-  have f2: "sbfun_io_eq (iterate i\<cdot>(\<Lambda> z. (innerFeedbackSum4SPF\<rightleftharpoons>((sb \<uplus> z)\<bar> {c1, c5})))) {c5}"
-    proof (induction i)
-      case 0
-      then show ?case
-        by(simp)
-    next
-      have f3: "sbDom\<cdot>z = {c5} \<Longrightarrow> sbDom\<cdot>((innerFeedbackSum4SPF\<rightleftharpoons>((sb \<uplus> z)\<bar> {c1, c5}))) = {c5}"
-        by (metis Int_insert_right domInnerFeedbackSum4SPF hidespfwell_helper ranInnerFeedbackSum4SPF ranInnerFeedbackSum4SPF_sb sbrestrict_sbdom sbunion_restrict)
-      case (Suc i)
-      then show ?case
-        apply(subst iterate_Suc)
-        apply(subst Abs_cfun_inverse2)
-         apply(subst t5, simp add: assms, simp)
-          by (smt domInnerFeedbackSum4SPF option.collapse ranInnerFeedbackSum4SPF ranInnerFeedbackSum4SPF_sb sbunion_restrict spfdom2sbdom spfran2sbdom)
-    qed       
-  show ?case 
+  then show ?case
     apply(subst iterate_Suc)
-    apply(simp)
+    apply(subst iterate_Suc)
     apply(subst (1) t4)
-     apply(simp_all add: f2 assms)
-      using Suc.IH by presburger
-qed
+     apply(simp add: t5 assms)
+     apply(simp add: t5 assms)
+      by presburger
+qed  
 
-lemma spf_gen_fix_sb_eq_lub: assumes "sbDom\<cdot>sb = {c1}" shows
-   "(\<Squnion>i. iterate (i)\<cdot>(\<Lambda> z. ([c5 \<mapsto> add\<cdot>(sb . c1)\<cdot>((appendElem2 0)\<cdot>(z . c5))]\<Omega>))\<cdot>({c5}^\<bottom>)) . c5
-    = (\<Squnion>i. iterate (i)\<cdot>(\<Lambda> z. ([c5 \<mapsto> add\<cdot>(sb . c1)\<cdot>((appendElem2 0)\<cdot>(z . c5))]\<Omega>))\<cdot>({c5}^\<bottom>) . c5)"
-   by (simp add: spf_feed_sb_inout1_lub_getch)
-     
+
+lemma t9: assumes "sbDom\<cdot>sb = {c1}" shows "iterate i\<cdot>(\<Lambda> z. add\<cdot>(sb . c1)\<cdot>(appendElem2 0\<cdot>z))\<cdot>\<epsilon> =
+            iterate i\<cdot>(\<Lambda> z. [c3 \<mapsto> sb . c1, c4 \<mapsto> appendElem2 0\<cdot>(z . c5), c5 \<mapsto> add\<cdot>(sb . c1)\<cdot>(appendElem2 0\<cdot>(z . c5))]\<Omega>)\<cdot>({c3, c4, c5}^\<bottom>) . c5"
+proof (induction i)
+  case 0
+  then show ?case
+    by simp
+  next
+  case (Suc i)
+  then show ?case
+    apply (unfold iterate_Suc)
+    apply(subst Abs_cfun_inverse2, simp)
+    apply(subst Abs_cfun_inverse2)
+    apply(subst t7, simp add: assms, simp)
+    apply(subst t22)
+    by presburger
+qed
+  
+(* eq lemmas *) 
+  
 lemma spf_gen_fix_sb_eq: assumes "sbDom\<cdot>sb = {c1}" shows
    "(gen_fix add (appendElem2 0))\<cdot>(sb . c1) = 
-  (\<Squnion>i. iterate (i)\<cdot>(\<Lambda> z. ([c5 \<mapsto> add\<cdot>(sb . c1)\<cdot>((appendElem2 0)\<cdot>(z . c5))]\<Omega>))\<cdot>({c5}^\<bottom>)) . c5"
-  apply(simp)
-  apply(subst spf_gen_fix_sb_eq_lub, simp add: assms)
-    using spf_feed_sb_inout1_iter_eq by auto
+    (\<Squnion>i. iterate (i)\<cdot>(\<Lambda> z. ([c3 \<mapsto> (sb . c1), c4 \<mapsto> (appendElem2 0\<cdot>(z . c5)), c5 \<mapsto> add\<cdot>(sb . c1)\<cdot>((appendElem2 0)\<cdot>(z . c5))]\<Omega>))\<cdot>({c3, c4, c5}^\<bottom>)) . c5"
+apply (subst sbgetch_lub)
+ apply(rule sbIterate_chain)
+  apply(simp add: t8 assms)
+by(simp add: t9 assms)
     
 lemma spf_spfFeedH_sb_eq: assumes "sbDom\<cdot>sb = {c1}" shows
-   "(\<Squnion>i. iter_sbfix (spfFeedH (spfRename innerSum4SPF [c5 \<mapsto> c2])) i {c5} sb) . c5 = 
-  (\<Squnion>i. iterate (i)\<cdot>(\<Lambda> z. (innerFeedbackSum4SPF\<rightleftharpoons>((sb \<uplus> z)\<bar> {c1, c5})))\<cdot>({c5}^\<bottom>)) . c5"
+   "(\<Squnion>i. iter_sbfix (spfFeedH (spfRename innerSum4SPF [c5 \<mapsto> c2])) i {c3, c4, c5} sb) . c5 = 
+    (\<Squnion>i. iterate (i)\<cdot>(\<Lambda> z. (innerFeedbackSum4SPF\<rightleftharpoons>((sb \<uplus> z)\<bar> {c1, c5})))\<cdot>({c3, c4, c5}^\<bottom>)) . c5"
   apply(simp add: spfFeedH_def)
-    by(simp add: domInnerFeedbackSum4SPF)
- 
+  by(simp add: domInnerFeedbackSum4SPF)
+  
 lemma iter_spfCompH3_eq_iter_sbfix_spfFeedH: assumes "sbDom\<cdot>sb = {c1}" shows
-  "(\<Squnion>i. iter_sbfix (spfFeedH (spfRename innerSum4SPF [c5 \<mapsto> c2])) i {c5} sb) . c5
-    =  (gen_fix add (appendElem2 0))\<cdot>(sb . c1)" 
-  apply(subst spf_gen_fix_sb_eq, simp add: assms)
-  apply(subst spf_spfFeedH_sb_eq, simp add: assms)
-    by (simp add: assms t2)
-      
-      
-section \<open> result \<close>
+  "(\<Squnion>i. iter_sbfix (spfFeedH (spfRename innerSum4SPF [c5 \<mapsto> c2])) i {c3, c4, c5} sb) . c5
+    =  (gen_fix add (appendElem2 0))\<cdot>(sb . c1)"
+proof - 
+  have f1: "sbfun_io_eq (\<Lambda> z. innerFeedbackSum4SPF\<rightleftharpoons>((sb \<uplus> z)\<bar>{c1, c5})) {c3, c4, c5}"
+    apply(subst Abs_cfun_inverse2)
+     apply(subst t6, simp_all add: assms)
+    apply(subst ranInnerFeedbackSum4SPF_sb)
+    using assms apply auto[1]
+      by (simp add: ranInnerFeedbackSum4SPF)
+  show ?thesis
+    apply(subst spf_gen_fix_sb_eq, simp add: assms)
+    apply(subst spf_spfFeedH_sb_eq, simp add: assms)
+    apply(subst sbgetch_lub)
+     apply(rule sbIterate_chain)
+      apply(simp add: f1)
+    apply(subst sbgetch_lub)
+     apply(rule sbIterate_chain)
+     apply(simp add: t8 assms sbdom_rep_eq)
+    by (simp add: assms t2)  
+qed
+  
+  
+section \<open>Final lemma\<close>  
+  
   
 lemma finalLemma: assumes "sbDom\<cdot>sb = spfDom\<cdot>sum4SPF" shows "(sum4SPF \<rightleftharpoons> sb) . c5 =  sum4\<cdot>(sb . c1)"
-proof -
+proof - 
   have f1: "{c1} = {c1, c5} - {c5}"
     by auto
   have f2: "sum4\<cdot>(sb . c1) = (gen_fix add (appendElem2 0))\<cdot>(sb . c1)"
@@ -374,10 +572,11 @@ proof -
     apply(subst spfFeedbackOperator2_iter_spfFeedH)
     apply(simp add: assms)
     apply(simp add: domInnerFeedbackSum4SPF ranInnerFeedbackSum4SPF)
-    apply(subst f1, simp, subst f1, simp) (* why isn't this directly solved by simp add: f1 or auto? *)
+    apply(simp add: f1)
     apply(subst f2)
     apply(subst iter_spfCompH3_eq_iter_sbfix_spfFeedH)
       by(simp_all add: assms)
 qed
-      
+  
+  
 end
